WIP

Std/Classes/BEq.lean
@@ -16,3 +16,40 @@ class PartialEquivBEq (α) [BEq α] : Prop where
   symm : (a : α) == b → b == a
   /-- Transitivity for `BEq`. If `a == b` and `b == c` then `a == c`. -/
   trans : (a : α) == b → b == c → a == c
+
+/-- `ReflBEq α` says that the `BEq` implementation is reflexive. -/
+class ReflBEq (α) [BEq α] : Prop where
+  /-- Reflexivity for `BEq`. -/
+  refl : (a : α) == a
+
+/-- `EquivBEq` says that the `BEq` implementation is an equivalence relation. -/
+class EquivBEq (α) [BEq α] extends PartialEquivBEq α, ReflBEq α : Prop
+
+@[simp]
+theorem BEq.refl [BEq α] [ReflBEq α] {a : α} : a == a :=
+  ReflBEq.refl
+
+theorem BEq.symm [BEq α] [PartialEquivBEq α] {a b : α} : a == b → b == a :=
+  PartialEquivBEq.symm
+
+theorem BEq.comm [BEq α] [PartialEquivBEq α] {a b : α} : (a == b) = (b == a) :=
+  Bool.eq_iff_iff.2 ⟨BEq.symm, BEq.symm⟩
+
+theorem BEq.symm_false [BEq α] [PartialEquivBEq α] {a b : α} : (a == b) = false → (b == a) = false :=
+  BEq.comm (α := α) ▸ id
+
+theorem BEq.trans [BEq α] [PartialEquivBEq α] {a b c : α} : a == b → b == c → a == c :=
+  PartialEquivBEq.trans
+
+theorem BEq.neq_of_neq_of_beq [BEq α] [PartialEquivBEq α] {a b c : α} :
+    (a == b) = false → b == c → (a == c) = false := by
+  refine fun h₁ h₂ => Bool.eq_false_iff.2 fun h₃ => Bool.eq_false_iff.1 h₁ (BEq.trans h₃ (BEq.symm h₂))
+
+theorem BEq.neq_of_beq_of_neq [BEq α] [PartialEquivBEq α] {a b c : α} :
+    a == b → (b == c) = false → (a == c) = false := by
+  refine fun h₁ h₂ => Bool.eq_false_iff.2 fun h₃ => Bool.eq_false_iff.1 h₂ (BEq.trans (BEq.symm h₁) h₃)
+
+instance (priority := low) [BEq α] [LawfulBEq α] : EquivBEq α where
+  refl := LawfulBEq.rfl
+  symm h := (beq_iff_eq _ _).2 <| Eq.symm <| (beq_iff_eq _ _).1 h
+  trans hab hbc := (beq_iff_eq _ _).2 <| ((beq_iff_eq _ _).1 hab).trans <| (beq_iff_eq _ _).1 hbc
