Std/Data/AList/Basic.lean
@@ -1,0 +1,631 @@
+/-
+Copyright (c) 2019 Microsoft Corporation. All rights reserved.
+Released under Apache 2.0 license as described in the file LICENSE.
+Authors: Leonardo de Moura, Mario Carneiro, Markus Himmel
+-/
+import Std.Classes.BEq
+
+universe v u
+
+variable {α : Type u} {β : α → Type v}
+
+namespace List
+
+@[elab_as_elim]
+theorem assoc_induction {motive : List (Σ a, β a) → Prop} (nil : motive [])
+    (cons : (k : α) → (v : β k) → (tail : List (Σ a, β a)) → motive tail → motive (⟨k, v⟩ :: tail)) :
+    (t : List (Σ a, β a)) → motive t
+  | [] => nil
+  | ⟨_, _⟩ :: _ => cons _ _ _ (assoc_induction nil cons _)
+
+/-- `O(n)`. Returns the first entry in the list whose key is equal to `a`. -/
+def findEntry? [BEq α] (a : α) : List (Σ a, β a) → Option (Σ a, β a)
+  | [] => none
+  | ⟨k, v⟩ :: es => bif k == a then some ⟨k, v⟩ else findEntry? a es
+
+@[simp] theorem findEntry?_nil [BEq α] {a : α} : ([] : List (Σ a, β a)).findEntry? a = none := rfl
+theorem findEntry?_cons [BEq α] {l : List (Σ a, β a)} {k a : α} {v : β k} :
+    (⟨k, v⟩ :: l).findEntry? a = bif k == a then some ⟨k, v⟩ else l.findEntry? a := rfl
+
+theorem findEntry?_cons_of_true [BEq α] {l : List (Σ a, β a)} {k a : α} {v : β k} (h : k == a) :
+    (⟨k, v⟩ :: l).findEntry? a = some ⟨k, v⟩ := by
+  simp [findEntry?, h]
+
+theorem findEntry?_cons_of_false [BEq α] {l : List (Σ a, β a)} {k a : α} {v : β k} (h : (k == a) = false) :
+    (⟨k, v⟩ :: l).findEntry? a = l.findEntry? a := by
+  simp [findEntry?, h]
+
+theorem findEntry?_eq_of_beq [BEq α] [EquivBEq α] {l : List (Σ a, β a)} {a a' : α} (h : a == a') :
+    l.findEntry? a = l.findEntry? a' := by
+  induction l using assoc_induction
+  · simp
+  · next k v l ih =>
+    cases h' : k == a
+    · have h₂ : (k == a') = false := BEq.neq_of_neq_of_beq h' h
+      rw [findEntry?_cons_of_false h', findEntry?_cons_of_false h₂, ih]
+    · rw [findEntry?_cons_of_true h', findEntry?_cons_of_true (BEq.trans h' h)]
+
+section
+
+variable {β : Type v}
+
+def findValue? [BEq α] (a : α) : List ((_ : α) × β) → Option β
+  | [] => none
+  | ⟨k, v⟩ :: l => bif k == a then some v else l.findValue? k
+
+
+
+@[simp] theorem findValue?_nil [BEq α] {a : α} : ([] : List ((_ : α) × β)).findValue? a = none := rfl
+theorem findValue?_cons [BEq α] {l : AssocList' α β} {k a : α} {v : β} :
+    (l.cons k v).find? a = bif k == a then some v else l.find? a := rfl
+
+theorem find?_cons_of_true [BEq α] {l : AssocList' α β} {k a : α} {v : β} (h : k == a) :
+    (l.cons k v).find? a = some v := by
+  simp [find?, h]
+
+theorem find?_cons_of_false [BEq α] {l : AssocList' α β} {k a : α} {v : β} (h : (k == a) = false) :
+    (l.cons k v).find? a = l.find? a := by
+  simp [find?, h]
+
+theorem find?_eq_findEntry? [BEq α] {l : AssocList' α β} {a : α} :
+    l.find? a = (l.findEntry? a).map (·.2) := by
+  induction l
+  · simp
+  · next k v es ih =>
+    cases h : k == a
+    · rw [findEntry?_cons_of_false h, find?_cons_of_false h, ih]
+    · rw [findEntry?_cons_of_true h, find?_cons_of_true h, Option.map_some']
+
+theorem find?_eq_of_beq [BEq α] [EquivBEq α] {l : AssocList' α β} {a a' : α} (h : a == a') :
+    l.find? a = l.find? a' := by
+  simp [find?_eq_findEntry?, findEntry?_eq_of_beq h]
+
+end
+
+def findKey? [BEq α] (a : α) : AssocList α β → Option α
+  | nil => none
+  | cons k _ es => bif k == a then some k else findKey? a es
+
+@[simp] theorem findKey?_nil [BEq α] {a : α} : (nil : AssocList α β).findKey? a = none := rfl
+theorem findKey?_cons [BEq α] {l : AssocList α β} {k a : α} {v : β k} :
+    (l.cons k v).findKey? a = bif k == a then some k else l.findKey? a := rfl
+
+theorem findKey?_cons_of_true [BEq α] {l : AssocList α β} {k a : α} {v : β k} (h : k == a) :
+    (l.cons k v).findKey? a = some k := by
+  simp [findKey?, h]
+
+theorem findKey?_cons_of_false [BEq α] {l : AssocList α β} {k a : α} {v : β k} (h : (k == a) = false) :
+    (l.cons k v).findKey? a = l.findKey? a := by
+  simp [findKey?, h]
+
+theorem findKey?_eq_findEntry? [BEq α] {l : AssocList α β} {a : α} :
+    l.findKey? a = (l.findEntry? a).map (·.1) := by
+  induction l
+  · simp
+  · next k v es ih =>
+    cases h : k == a
+    · rw [findEntry?_cons_of_false h, findKey?_cons_of_false h, ih]
+    · rw [findEntry?_cons_of_true h, findKey?_cons_of_true h, Option.map_some']
+
+theorem findKey?_eq_of_beq [BEq α] [EquivBEq α] {l : AssocList α β} {a a' : α} (h : a == a') :
+    l.findKey? a = l.findKey? a' := by
+  simp [findKey?_eq_findEntry?, findEntry?_eq_of_beq h]
+
+def contains [BEq α] (a : α) : AssocList α β → Bool
+  | nil => false
+  | cons k _ l => k == a || l.contains a
+
+@[simp] theorem contains_nil [BEq α] {a : α} : (nil : AssocList α β).contains a = false := rfl
+@[simp] theorem contains_cons [BEq α] {l : AssocList α β} {k a : α} {v : β k} :
+    (l.cons k v).contains a = (k == a || l.contains a) := rfl
+
+theorem contains_cons_eq_false [BEq α] {l : AssocList α β} {k a : α} {v : β k} :
+    ((l.cons k v).contains a = false) ↔ ((k == a) = false) ∧ (l.contains a = false) := by
+  rw [Bool.eq_iff_iff]
+  simp [contains_cons, not_or]
+
+theorem contains_cons_eq_true [BEq α] {l : AssocList α β} {k a : α} {v : β k} :
+    ((l.cons k v).contains a) ↔ (k == a) ∨ (l.contains a) := by
+  rw [Bool.eq_iff_iff]
+  simp [contains_cons]
+
+theorem contains_cons_of_beq [BEq α] {l : AssocList α β} {k a : α} {v : β k} (h : k == a) :
+    (l.cons k v).contains a := contains_cons_eq_true.2 <| Or.inl h
+
+@[simp]
+theorem contains_cons_self [BEq α] [EquivBEq α] {l : AssocList α β} {k : α} {v : β k} :
+    (l.cons k v).contains k := contains_cons_of_beq BEq.refl
+
+theorem contains_cons_of_contains [BEq α] {l : AssocList α β} {k a : α} {v : β k} (h : l.contains a) :
+    (l.cons k v).contains a := contains_cons_eq_true.2 <| Or.inr h
+
+theorem contains_of_contains_cons [BEq α] {l : AssocList α β} {k a : α} {v : β k} (h₁ : (l.cons k v).contains a)
+    (h₂ : (k == a) = false) : l.contains a := by
+  rcases (contains_cons_eq_true.1 h₁) with (h|h)
+  · exact False.elim (Bool.eq_false_iff.1 h₂ h)
+  · exact h
+
+theorem contains_eq_isSome_findEntry? [BEq α] {l : AssocList α β} {a : α} :
+    l.contains a = (l.findEntry? a).isSome := by
+  induction l
+  · simp
+  · next k v l ih =>
+    cases h : k == a
+    · simp [findEntry?_cons_of_false h, h, ih]
+    · simp [findEntry?_cons_of_true h, h]
+
+theorem contains_eq_isSome_find? {β : Type v} [BEq α] {l : AssocList' α β} {a : α} :
+    l.contains a = (l.find? a).isSome := by
+  simp [contains_eq_isSome_findEntry?, find?_eq_findEntry?]
+
+theorem contains_eq_isSome_findKey? [BEq α] {l : AssocList α β} {a : α} :
+    l.contains a = (l.findKey? a).isSome := by
+  simp [contains_eq_isSome_findEntry?, findKey?_eq_findEntry?]
+
+theorem contains_eq_of_beq [BEq α] [EquivBEq α] {l : AssocList α β} {a b : α} (h : a == b) :
+    l.contains a = l.contains b := by
+  simp [contains_eq_isSome_findEntry?, findEntry?_eq_of_beq h]
+
+theorem contains_of_beq [BEq α] [EquivBEq α] {l : AssocList α β} {a b : α} (hla : l.contains a) (hab : a == b) :
+    l.contains b := by
+  rwa [← contains_eq_of_beq hab]
+
+def findEntry [BEq α] (l : AssocList α β) (a : α) (h : l.contains a) : Σ a, β a :=
+  (l.findEntry? a).get <| contains_eq_isSome_findEntry?.symm.trans h
+
+theorem findEntry?_eq_some_findEntry [BEq α] {l : AssocList α β} {a : α} (h : l.contains a) :
+    l.findEntry? a = some (l.findEntry a h) := by
+  simp [findEntry]
+
+theorem findEntry_cons_of_beq [BEq α] {l : AssocList α β} {k a : α} {v : β k} (h : k == a) :
+    (l.cons k v).findEntry a (contains_cons_of_beq h) = ⟨k, v⟩ := by
+  simp [findEntry, findEntry?_cons_of_true h]
+
+@[simp]
+theorem findEntry_cons_self [BEq α] [EquivBEq α] {l : AssocList α β} {k : α} {v : β k} :
+    (l.cons k v).findEntry k contains_cons_self = ⟨k, v⟩ :=
+  findEntry_cons_of_beq BEq.refl
+
+theorem findEntry_cons_of_false [BEq α] {l : AssocList α β} {k a : α} {v : β k} {h₁ : (l.cons k v).contains a}
+    (h₂ : (k == a) = false) : (l.cons k v).findEntry a h₁ = l.findEntry a (contains_of_contains_cons h₁ h₂) := by
+  simp [findEntry, findEntry?_cons_of_false h₂]
+
+def findKey [BEq α] (l : AssocList α β) (a : α) (h : l.contains a) : α :=
+  (l.findKey? a).get <| contains_eq_isSome_findKey?.symm.trans h
+
+theorem findKey?_eq_some_findKey [BEq α] {l : AssocList α β} {a : α} (h : l.contains a) :
+    l.findKey? a = some (l.findKey a h) := by
+  simp [findKey]
+
+theorem findKey_cons_of_beq [BEq α] {l : AssocList α β} {k a : α} {v : β k} (h : k == a) :
+    (l.cons k v).findKey a (contains_cons_of_beq h) = k := by
+  simp [findKey, findKey?_cons_of_true h]
+
+@[simp]
+theorem findKey_cons_self [BEq α] [EquivBEq α] {l : AssocList α β} {k : α} {v : β k} :
+    (l.cons k v).findKey k contains_cons_self = k :=
+  findKey_cons_of_beq BEq.refl
+
+theorem findKey_cons_of_false [BEq α] {l : AssocList α β} {k a : α} {v : β k} {h₁ : (l.cons k v).contains a}
+    (h₂ : (k == a) = false) : (l.cons k v).findKey a h₁ = l.findKey a (contains_of_contains_cons h₁ h₂) := by
+  simp [findKey, findKey?_cons_of_false h₂]
+
+theorem findKey_beq [BEq α] {l : AssocList α β} {a : α} {h : l.contains a} : l.findKey a h == a := by
+  induction l
+  · simp at h
+  · next k v t ih =>
+    cases h' : k == a
+    · rw [findKey_cons_of_false h']
+      exact @ih (contains_of_contains_cons h h')
+    · rwa [findKey_cons_of_beq h']
+
+section
+
+variable {β : Type v}
+
+def find [BEq α] (l : AssocList' α β) (a : α) (h : l.contains a) : β :=
+  (l.find? a).get <| contains_eq_isSome_find?.symm.trans h
+
+theorem find?_eq_some_find [BEq α] {l : AssocList' α β} {a : α} (h : l.contains a) :
+    l.find? a = some (l.find a h) := by
+  simp [find]
+
+theorem find_cons_of_beq [BEq α] {l : AssocList' α β} {k a : α} {v : β} (h : k == a) :
+    (l.cons k v).find a (contains_cons_of_beq h) = v := by
+  simp [find, find?_cons_of_true h]
+
+@[simp]
+theorem find_cons_self [BEq α] [EquivBEq α] {l : AssocList' α β} {k : α} {v : β} :
+    (l.cons k v).find k contains_cons_self = v :=
+  find_cons_of_beq BEq.refl
+
+theorem find_cons_of_false [BEq α] {l : AssocList' α β} {k a : α} {v : β} {h₁ : (l.cons k v).contains a}
+    (h₂ : (k == a) = false) : (l.cons k v).find a h₁ = l.find a (contains_of_contains_cons h₁ h₂) := by
+  simp [find, find?_cons_of_false h₂]
+
+end
+
+def replace [BEq α] (a : α) (b : β a) : AssocList α β → AssocList α β
+  | nil => nil
+  | cons k v l => bif k == a then cons a b l else cons k v (replace a b l)
+
+@[simp] theorem replace_nil [BEq α] {a : α} {b : β a} : nil.replace a b = nil := rfl
+theorem replace_cons [BEq α] {l : AssocList α β} {k a : α} {v : β k} {b : β a} :
+    (l.cons k v).replace a b = bif k == a then l.cons a b else (l.replace a b).cons k v := rfl
+
+theorem replace_cons_of_true [BEq α] {l : AssocList α β} {k a : α} {v : β k} {b : β a} (h : k == a) :
+    (l.cons k v).replace a b = l.cons a b := by
+  simp [replace, h]
+
+theorem replace_cons_of_false [BEq α] {l : AssocList α β} {k a : α} {v : β k} {b : β a} (h : (k == a) = false) :
+    (l.cons k v).replace a b = (l.replace a b).cons k v := by
+  simp [replace, h]
+
+theorem replace_of_contains_eq_false [BEq α] {l : AssocList α β} {a : α} {b : β a} (h : l.contains a = false) :
+    l.replace a b = l := by
+  induction l
+  · simp
+  · next k v l ih =>
+    rw [contains_cons_eq_false] at h
+    rw [replace_cons_of_false h.1, ih h.2]
+
+theorem findEntry?_replace_of_contains_eq_false [BEq α] {l : AssocList α β} {k a : α} {b : β a}
+    (hl : l.contains a = false) : (l.replace a b).findEntry? k = l.findEntry? k := by
+  rw [replace_of_contains_eq_false hl]
+
+theorem findEntry?_replace_of_false [BEq α] [EquivBEq α] {l : AssocList α β} {k a : α} {b : β a}
+    (h : (k == a) = false) : (l.replace a b).findEntry? k = l.findEntry? k := by
+  induction l
+  · simp
+  · next k' v' l ih =>
+    cases h' : k' == a
+    · rw [replace_cons_of_false h', findEntry?_cons, findEntry?_cons, ih]
+    · rw [replace_cons_of_true h']
+      have hk : (k' == k) = false := BEq.neq_of_beq_of_neq h' (BEq.symm_false h)
+      simp [findEntry?_cons_of_false (BEq.symm_false h), findEntry?_cons_of_false hk]
+
+theorem findEntry?_replace_of_true [BEq α] [EquivBEq α] {l : AssocList α β} {k a : α} {b : β a} (hl : l.contains a = true)
+    (h : k == a) : (l.replace a b).findEntry? k = some ⟨a, b⟩ := by
+  induction l
+  · simp at hl
+  · next k' v' l ih =>
+    cases hk'a : k' == a
+    · rw [replace_cons_of_false hk'a]
+      have hk'k : (k' == k) = false := BEq.neq_of_neq_of_beq hk'a (BEq.symm h)
+      rw [findEntry?_cons_of_false hk'k]
+      exact ih (contains_of_contains_cons hl hk'a)
+    · rw [replace_cons_of_true hk'a, findEntry?_cons_of_true (BEq.symm h)]
+
+section
+
+variable {β : Type v}
+
+theorem find?_replace_of_contains_eq_false [BEq α] {l : AssocList' α β} {k a : α} {b : β}
+    (hl : l.contains a = false) : (l.replace a b).find? k = l.find? k := by
+  simp [find?_eq_findEntry?, findEntry?_replace_of_contains_eq_false hl]
+
+theorem find?_replace_of_false [BEq α] [EquivBEq α] {l : AssocList' α β} {k a : α} {b : β}
+    (h : (k == a) = false) : (l.replace a b).find? k = l.find? k := by
+  simp [find?_eq_findEntry?, findEntry?_replace_of_false h]
+
+theorem find?_replace_of_true [BEq α] [EquivBEq α] {l : AssocList' α β} {k a : α} {b : β}
+    (hl : l.contains a = true) (h : k == a) : (l.replace a b).find? k = some b := by
+  simp [find?_eq_findEntry?, findEntry?_replace_of_true hl h]
+
+end
+
+theorem findKey?_replace_of_contains_eq_false [BEq α] {l : AssocList α β} {k a : α} {b : β a}
+    (hl : l.contains a = false) : (l.replace a b).findKey? k = l.findKey? k := by
+  simp [findKey?_eq_findEntry?, findEntry?_replace_of_contains_eq_false hl]
+
+theorem findKey?_replace_of_false [BEq α] [EquivBEq α] {l : AssocList α β} {k a : α} {b : β a}
+    (h : (k == a) = false) : (l.replace a b).findKey? k = l.findKey? k := by
+  simp [findKey?_eq_findEntry?, findEntry?_replace_of_false h]
+
+theorem findKey?_replace_of_true [BEq α] [EquivBEq α] {l : AssocList α β} {k a : α} {b : β a}
+    (hl : l.contains a = true) (h : (k == a)) : (l.replace a b).findKey? k = some a := by
+  simp [findKey?_eq_findEntry?, findEntry?_replace_of_true hl h]
+
+theorem findKey?_replace [BEq α] [EquivBEq α] {l : AssocList α β} {k a : α} {b : β a} :
+    (l.replace a b).findKey? k = bif l.contains a && k == a then some a else l.findKey? k := by
+  cases hl : l.contains a
+  · simp [findKey?_replace_of_contains_eq_false hl]
+  · cases h : k == a
+    · simp [findKey?_replace_of_false h]
+    · simp [findKey?_replace_of_true hl h]
+
+@[simp]
+theorem contains_replace [BEq α] [EquivBEq α] {l : AssocList α β} {k a : α} {b : β a} :
+    (l.replace a b).contains k = l.contains k := by
+  cases h : l.contains a && k == a
+  · rw [contains_eq_isSome_findKey?, findKey?_replace, h, cond_false, contains_eq_isSome_findKey?]
+  · rw [contains_eq_isSome_findKey?, findKey?_replace, h, cond_true, Option.isSome_some, Eq.comm]
+    rw [Bool.and_eq_true] at h
+    exact contains_of_beq h.1 (BEq.symm h.2)
+
+def erase [BEq α] (a : α) : AssocList α β → AssocList α β
+  | nil => nil
+  | cons k v l => bif k == a then l else cons k v (l.erase a)
+
+@[simp] theorem erase_nil [BEq α] {a : α} : (nil : AssocList α β).erase a = nil := rfl
+theorem erase_cons [BEq α] {l : AssocList α β} {k a : α} {v : β k} :
+    (l.cons k v).erase a = bif k == a then l else cons k v (l.erase a) := rfl
+
+theorem erase_cons_of_beq [BEq α] {l : AssocList α β} {k a : α} {v : β k} (h : k == a) :
+    (l.cons k v).erase a = l :=
+  by simp [erase_cons, h]
+
+@[simp]
+theorem erase_cons_self [BEq α] [EquivBEq α] {l : AssocList α β} {k : α} {v : β k} :
+    (l.cons k v).erase k = l :=
+  erase_cons_of_beq BEq.refl
+
+theorem erase_cons_of_false [BEq α] {l : AssocList α β} {k a : α} {v : β k} (h : (k == a) = false) :
+    (l.cons k v).erase a = (l.erase a).cons k v := by
+  simp [erase_cons, h]
+
+-- TODO: erase+replace
+
+/--
+`O(n)`. Convert an `AssocList α β` to the list of keys in appearance order.
+-/
+def keys : AssocList α β → List α
+  | nil => []
+  | cons k _ l => k :: (keys l)
+
+@[simp] theorem keys_nil : (nil : AssocList α β).keys = [] := rfl
+@[simp] theorem keys_cons {l : AssocList α β} {k : α} {v : β k} : (l.cons k v).keys = k :: l.keys := rfl
+
+theorem contains_eq_keys_contains [BEq α] [EquivBEq α] {l : AssocList α β} {a : α} :
+    l.contains a = l.keys.contains a := by
+  induction l
+  · rfl
+  · next k _ l ih =>
+    simp [ih, BEq.comm]
+
+/-- The well-formedness predicate for `AssocList` says that keys are pairwise distinct. -/
+structure WF [BEq α] (l : AssocList α β) : Prop where
+  distinct : l.keys.Pairwise fun a b => (a == b) = false
+
+@[simp]
+theorem WF_nil [BEq α] : (nil : AssocList α β).WF :=
+  ⟨by simp⟩
+
+open List
+
+theorem WF_of_sublist_keys [BEq α] {l l' : AssocList α β} (h : l'.keys <+ l.keys) : l.WF → l'.WF :=
+  fun ⟨h'⟩ => ⟨h'.sublist h⟩
+
+theorem WF_of_keys_eq [BEq α] {l l' : AssocList α β} (h : l.keys = l'.keys) : l.WF → l'.WF :=
+  WF_of_sublist_keys (h ▸ Sublist.refl _)
+
+theorem contains_iff_exists [BEq α] [EquivBEq α] {l : AssocList α β} {a : α} :
+    l.contains a ↔ ∃ a' ∈ l.keys, a == a' := by
+  rw [contains_eq_keys_contains, List.contains_iff_exists_beq]
+
+theorem contains_eq_false_iff_forall [BEq α] [EquivBEq α] {l : AssocList α β} {a : α} :
+    (l.contains a) = false ↔ ∀ a' ∈ l.keys, (a == a') = false := by
+  simp only [Bool.eq_false_iff, ne_eq, contains_iff_exists, not_exists, not_and]
+
+@[simp]
+theorem WF_cons_iff [BEq α] [EquivBEq α] {l : AssocList α β} {k : α} {v : β k} :
+    (l.cons k v).WF ↔ l.WF ∧ (l.contains k) = false := by
+  refine ⟨fun ⟨h⟩ => ?_, fun ⟨⟨h₁⟩, h₂⟩ => ⟨?_⟩⟩
+  · rw [keys_cons, List.pairwise_cons] at h
+    exact ⟨⟨h.2⟩, contains_eq_false_iff_forall.2 h.1⟩
+  · rw [keys_cons, List.pairwise_cons, ← contains_eq_false_iff_forall]
+    exact ⟨h₂, h₁⟩
+
+theorem WF_cons [BEq α] [EquivBEq α] {l : AssocList α β} {k : α} {v : β k} (h : l.contains k = false) :
+    l.WF → (l.cons k v).WF :=
+  fun h' => WF_cons_iff.mpr ⟨h', h⟩
+
+theorem WF_replace [BEq α] [EquivBEq α] {l : AssocList α β} {k : α} {v : β k} (h : l.WF) : (l.replace k v).WF := by
+  induction l
+  · simp
+  · next k' v' l ih =>
+    rw [WF_cons_iff] at h
+    cases hk'k : k' == k
+    · rw [replace_cons_of_false hk'k, WF_cons_iff]
+      refine ⟨ih h.1, ?_⟩
+      simpa using h.2
+    · rw [replace_cons_of_true hk'k, WF_cons_iff]
+      refine ⟨h.1, ?_⟩
+      simpa [contains_eq_of_beq (BEq.symm hk'k)] using h.2
+
+def insert [BEq α] (l : AssocList α β) (k : α) (v : β k) : AssocList α β :=
+  bif l.contains k then l.replace k v else l.cons k v
+
+theorem insert_of_contains [BEq α] {l : AssocList α β} {k : α} {v : β k} (h : l.contains k) :
+    l.insert k v = l.replace k v := by
+  simp [insert, h]
+
+theorem insert_of_contains_eq_false [BEq α] {l : AssocList α β} {k : α} {v : β k} (h : l.contains k = false) :
+    l.insert k v = l.cons k v := by
+  simp [insert, h]
+
+theorem WF_insert [BEq α] [EquivBEq α] {l : AssocList α β} {k : α} {v : β k} (h : l.WF) : (l.insert k v).WF := by
+  cases h' : l.contains k
+  · rw [insert_of_contains_eq_false h', WF_cons_iff]
+    exact ⟨h, h'⟩
+  · rw [insert_of_contains h']
+    exact WF_replace h
+
+section
+
+variable {β : Type v}
+
+theorem find?_insert_of_beq [BEq α] [EquivBEq α] {l : AssocList' α β} {k a : α} {v : β} (h : k == a) :
+    (l.insert k v).find? a = some v := by
+  cases h' : l.contains k
+  · rw [insert_of_contains_eq_false h', find?_cons_of_true h]
+  · rw [insert_of_contains h', find?_replace_of_true h' (BEq.symm h)]
+
+theorem find?_insert_of_self [BEq α] [EquivBEq α] {l : AssocList' α β} {k : α} {v : β} :
+    (l.insert k v).find? k = some v :=
+  find?_insert_of_beq BEq.refl
+
+theorem find?_insert_of_false [BEq α] [EquivBEq α] {l : AssocList' α β} {k a : α} {v : β} (h : (k == a) = false) :
+    (l.insert k v).find? a = l.find? a := by
+  cases h' : l.contains k
+  · rw [insert_of_contains_eq_false h', find?_cons_of_false h]
+  · rw [insert_of_contains h', find?_replace_of_false (BEq.symm_false h)]
+
+-- TODO: would this be a reasonable simp lemma?
+theorem find?_insert [BEq α] [EquivBEq α] {l : AssocList' α β} {k a : α} {v : β} :
+    (l.insert k v).find? a = bif k == a then some v else l.find? a := by
+  cases h : k == a
+  · simp [find?_insert_of_false h, h]
+  · simp [find?_insert_of_beq h, h]
+
+end
+
+-- TODO: Unify order in `bif k == a` vs. `bif a == k`.
+theorem findKey?_insert_of_contains [BEq α] [EquivBEq α] {l : AssocList α β} {k a : α} {v : β k}
+    (h : l.contains k) : (l.insert k v).findKey? a = bif k == a then some k else l.findKey? a := by
+  simp [insert_of_contains h, findKey?_replace, h, BEq.comm]
+
+theorem findKey?_insert_of_contains_eq_false [BEq α] [EquivBEq α] {l : AssocList α β} {k a : α} {v : β k}
+    (hl : (l.contains k) = false) :
+    (l.insert k v).findKey? a = bif k == a then some k else l.findKey? a := by
+  simp [insert_of_contains_eq_false hl, findKey?_cons]
+
+theorem findKey?_insert [BEq α] [EquivBEq α] {l : AssocList α β} {k a : α} {v : β k} :
+    (l.insert k v).findKey? a = bif k == a then some k else l.findKey? a := by
+  cases hl : l.contains k
+  · simp [findKey?_insert_of_contains_eq_false hl, hl]
+  · simp [findKey?_insert_of_contains hl]
+
+-- TODO: results about findEntry?+insert
+
+@[simp]
+theorem contains_insert [BEq α] [EquivBEq α] {l : AssocList α β} {k a : α} {v : β k} :
+    (l.insert k v).contains a = ((k == a) || l.contains a) := by
+  rw [contains_eq_isSome_findKey?, contains_eq_isSome_findKey?, findKey?_insert]
+  cases k == a
+  · simp
+  · simp
+
+theorem contains_insert_of_beq [BEq α] [EquivBEq α] {l : AssocList α β} {k a : α} {v : β k} (h : k == a) :
+    (l.insert k v).contains a := by
+  simp [h]
+
+@[simp]
+theorem contains_insert_self [BEq α] [EquivBEq α] {l : AssocList α β} {k : α} {v : β k} :
+    (l.insert k v).contains k :=
+  contains_insert_of_beq BEq.refl
+
+@[simp]
+theorem keys_erase [BEq α] [EquivBEq α] {l : AssocList α β} {k : α} :
+    (l.erase k).keys = l.keys.erase k := by
+  induction l
+  · rfl
+  · next k' v' l ih =>
+    simp only [erase_cons, keys_cons, List.erase_cons]
+    cases k' == k
+    · simp [ih]
+    · simp [ih]
+
+theorem WF_erase [BEq α] [EquivBEq α] {l : AssocList α β} {k : α} : l.WF → (l.erase k).WF := by
+  apply WF_of_sublist_keys (by simpa using erase_sublist' _ _)
+
+theorem findEntry?_erase_self [BEq α] [EquivBEq α] {l : AssocList α β} {k : α} (h : l.WF) :
+    (l.erase k).findEntry? k = none := by
+  induction l
+  · simp
+  · next k' v' t ih =>
+    cases h' : k' == k
+    · rw [erase_cons_of_false h', findEntry?_cons_of_false h']
+      exact ih (WF_cons_iff.1 h).1
+    · rw [erase_cons_of_beq h', ← Option.not_isSome_iff_eq_none, Bool.not_eq_true,
+        ← contains_eq_isSome_findEntry?, ← contains_eq_of_beq h']
+      exact (WF_cons_iff.1 h).2
+
+theorem findEntry?_erase_of_beq [BEq α] [EquivBEq α] {l : AssocList α β} {k a : α} (hl : l.WF)
+    (hka : k == a) : (l.erase k).findEntry? a = none := by
+  rw [← findEntry?_eq_of_beq hka, findEntry?_erase_self hl]
+
+theorem findEntry?_erase_of_false [BEq α] [EquivBEq α] {l : AssocList α β} {k a : α}
+    (hka : (k == a) = false) : (l.erase k).findEntry? a = l.findEntry? a := by
+  induction l
+  · simp
+  · next k' v' t ih =>
+    cases h' : k' == k
+    · rw [erase_cons_of_false h']
+      cases h'' : k' == a
+      · rw [findEntry?_cons_of_false h'', ih, findEntry?_cons_of_false h'']
+      · rw [findEntry?_cons_of_true h'', findEntry?_cons_of_true h'']
+    · rw [erase_cons_of_beq h']
+      have hx : (k' == a) = false := BEq.neq_of_beq_of_neq h' hka
+      rw [findEntry?_cons_of_false hx]
+
+theorem findEntry?_erase [BEq α] [EquivBEq α] {l : AssocList α β} {k a : α} (hl : l.WF) :
+    (l.erase k).findEntry? a = bif k == a then none else l.findEntry? a := by
+  cases h : k == a
+  · simp [findEntry?_erase_of_false h, h]
+  · simp [findEntry?_erase_of_beq hl h, h]
+
+section
+
+variable {β : Type v}
+
+theorem find?_erase_self [BEq α] [EquivBEq α] {l : AssocList' α β} {k : α} (h : l.WF) :
+    (l.erase k).find? k = none := by
+  simp [find?_eq_findEntry?, findEntry?_erase_self h]
+
+theorem find?_erase_of_beq [BEq α] [EquivBEq α] {l : AssocList' α β} {k a : α} (hl : l.WF)
+    (hka : k == a) : (l.erase k).find? a = none := by
+  simp [find?_eq_findEntry?, findEntry?_erase_of_beq hl hka]
+
+theorem find?_erase_of_false [BEq α] [EquivBEq α] {l : AssocList' α β} {k a : α}
+    (hka : (k == a) = false) : (l.erase k).find? a = l.find? a := by
+  simp [find?_eq_findEntry?, findEntry?_erase_of_false hka]
+
+theorem find?_erase [BEq α] [EquivBEq α] {l : AssocList' α β} {k a : α} (hl : l.WF) :
+    (l.erase k).find? a = bif k == a then none else l.find? a := by
+  simp [find?_eq_findEntry?, findEntry?_erase hl, apply_bif (Option.map _)]
+
+end
+
+theorem findKey?_erase_self [BEq α] [EquivBEq α] {l : AssocList α β} {k : α} (h : l.WF) :
+    (l.erase k).findKey? k = none := by
+  simp [findKey?_eq_findEntry?, findEntry?_erase_self h]
+
+theorem findKey?_erase_of_beq [BEq α] [EquivBEq α] {l : AssocList α β} {k a : α} (hl : l.WF)
+    (hka : k == a) : (l.erase k).findKey? a = none := by
+  simp [findKey?_eq_findEntry?, findEntry?_erase_of_beq hl hka]
+
+theorem findKey?_erase_of_false [BEq α] [EquivBEq α] {l : AssocList α β} {k a : α}
+    (hka : (k == a) = false) : (l.erase k).findKey? a = l.findKey? a := by
+  simp [findKey?_eq_findEntry?, findEntry?_erase_of_false hka]
+
+theorem findKey?_erase [BEq α] [EquivBEq α] {l : AssocList α β} {k a : α} (hl : l.WF) :
+    (l.erase k).findKey? a = bif k == a then none else l.findKey? a := by
+  simp [findKey?_eq_findEntry?, findEntry?_erase hl, apply_bif (Option.map _)]
+
+theorem contains_erase_self [BEq α] [EquivBEq α] {l : AssocList α β} {k : α} (h : l.WF) :
+    (l.erase k).contains k = false := by
+  simp [contains_eq_isSome_findEntry?, findEntry?_erase_self h]
+
+theorem contains_erase_of_beq [BEq α] [EquivBEq α] {l : AssocList α β} {k a : α} (hl : l.WF)
+    (hka : k == a) : (l.erase k).contains a = false := by
+  rw [← contains_eq_of_beq hka, contains_erase_self hl]
+
+theorem contains_erase_of_false [BEq α] [EquivBEq α] {l : AssocList α β} {k a : α}
+    (hka : (k == a) = false) : (l.erase k).contains a = l.contains a := by
+  simp [contains_eq_isSome_findEntry?, findEntry?_erase_of_false hka]
+
+theorem contains_erase [BEq α] [EquivBEq α] {l : AssocList α β} {k a : α} (hl : l.WF) :
+    (l.erase k).contains a = bif k == a then false else l.contains a := by
+  simp [contains_eq_isSome_findEntry?, findEntry?_erase hl, apply_bif Option.isSome]
+
+-- TODO: Technically this should be true without assuming l.WF
+theorem contains_of_contains_erase [BEq α] [EquivBEq α] {l : AssocList α β} {k a : α} (hl : l.WF)
+    (h : (l.erase k).contains a) : l.contains a := by
+  cases hka : k == a
+  · rwa [contains_erase_of_false hka] at h
+  · simp [contains_erase_of_beq hl hka] at h
+
+-- TODO: results about combining modification operations
+
+end List
